theories/goedel/goedel1.v
@@ -269,7 +269,7 @@ apply ( freeVarCodeSysPrf _ _ _ _ _ _ _ _ freeVarRepT _ H6).
            destruct (eq_nat_dec 1 0) as [e|n].
            ++ discriminate e.
            ++ induction
-               (In_dec eq_nat_dec 1 (freeVarT LNN
+               (In_dec eq_nat_dec 1 (freeVarT 
                                        (codeNatToTerm.natToTermLNN codeX)))
                  as [a | _]. 
               ** elim (closedNatToTerm _ _ a).
