theories/ordinals/Ackermann/folProp.v
@@ -948,7 +948,7 @@ Search substF.
   (substF3 (substF6 e v1 t1 v2 t2 v3 t3 v4 t4 v5 t5 v6 t6)
      v7 t7 v8 t8 v9 t9).
 
-About freeVarF.
 
 #[global] Arguments freeVarF {L} _.
-
+#[global] Arguments freeVarT {L} _.
+#[global] Arguments freeVarTs {L n} _.
